reorganize code from sbox example into different files

cava/arrow-examples/Aes/sbox_canright.v
@@ -16,78 +16,10 @@
 
 From Coq Require Import Arith Eqdep_dec Vector Lia NArith Omega String Ndigits.
 From Arrow Require Import Category Arrow.
-From Cava Require Import Arrow.ArrowExport BitArithmetic.
+From Cava Require Import Arrow.ArrowExport Arrow.CircuitFunctionalEquivalence
+     BitArithmetic Tactics VectorUtils.
 
 From ArrowExamples Require Import Combinators Aes.pkg Aes.sbox_canright_pkg.
-
-Inductive circuit_equiv: forall i o, Circuit i o -> (denote_kind i -> denote_kind o) -> Prop :=
-  | Composition_equiv: forall x y z c1 c2 r1 r2 r,
-    circuit_equiv x y c1 r1 ->
-    circuit_equiv y z c2 r2 ->
-    (forall a:denote_kind x, r a = r2 (r1 a) ) ->
-    circuit_equiv x z (Composition _ _ _ c1 c2) r
-
-  | Uncancell_equiv: forall x,
-    circuit_equiv x (Tuple Unit x) (Structural (Uncancell x)) (fun a => (tt, a))
-  | Uncancelr_equiv: forall x,
-    circuit_equiv x (Tuple x Unit) (Structural (Uncancelr x)) (fun a => (a, tt))
-
-  | Cancell_equiv: forall x,
-    circuit_equiv (Tuple Unit x) x (Structural (Cancell x)) (fun a => snd a)
-  | Cancelr_equiv: forall x,
-    circuit_equiv (Tuple x Unit) x (Structural (Cancelr x)) (fun a => fst a)
-
-  | First_equiv: forall x y z c r r1,
-    circuit_equiv x y c r1 ->
-    (forall a, r a = (r1 (fst a), snd a)) ->
-    circuit_equiv (Tuple x z) (Tuple y z) (First x y z c) r
-
-  | Second_equiv: forall x y z c r r1,
-    circuit_equiv x y c r1 ->
-    (forall a, r a = (fst a, r1 (snd a))) ->
-    circuit_equiv (Tuple z x) (Tuple z y) (Second x y z c) r
-
-  | Swap_equiv: forall x y,
-    circuit_equiv (Tuple x y) (Tuple y x) (Structural (Swap x y)) (fun a => (snd a, fst a))
-  | Drop_equiv: forall x,
-    circuit_equiv x Unit (Structural (Drop x)) (fun a => tt)
-  | Copy_equiv: forall x,
-    circuit_equiv x (Tuple x x) (Structural (Copy x)) (fun a => (a,a))
-
-  | Assoc_equiv: forall x y z,
-    circuit_equiv (Tuple (Tuple x y) z) (Tuple x (Tuple y z))
-    (Structural (Assoc x y z)) (fun i => (fst (fst i), (snd (fst i), snd i)))
-  | Unassoc_equiv: forall x y z,
-    circuit_equiv (Tuple x (Tuple y z)) (Tuple (Tuple x y) z)
-    (Structural (Unassoc x y z)) (fun i => ((fst i, fst (snd i)), snd (snd i)))
-
-  | Id_equiv: forall x,
-    circuit_equiv x x (Structural (Arrow.Id x)) (fun a => a)
-
-  | Map_equiv: forall x y n c r r1,
-    circuit_equiv x y c r1 ->
-    (forall v, r v = Vector.map r1 v) ->
-    circuit_equiv (Vector x n) (Vector y n) (Map x y n c) r
-
-  | Resize_equiv: forall x n nn,
-    circuit_equiv (Vector x n) (Vector x nn) (Resize x n nn)
-      (fun v => resize_default (kind_default _) nn v)
-
-  | Primtive_equiv: forall p,
-    circuit_equiv (primitive_input p) (primitive_output p) (CircuitArrow.Primitive p) (combinational_evaluation' (CircuitArrow.Primitive p))
-
-  (* | Any_equiv: forall i o c, *)
-  (*   circuit_equiv i o c (combinational_evaluation' c) *)
-  .
-
-(*   (1* contains subcircuits *1) *)
-(*   | First: forall x y z, Circuit x y -> Circuit (Tuple x z) (Tuple y z) *)
-(*   | Second: forall x y z, Circuit x y -> Circuit (Tuple z x) (Tuple z y) *)
-(*   | Loopr: forall x y z, Circuit (Tuple x z) (Tuple y z) -> Circuit x y *)
-(*   | Loopl: forall x y z, Circuit (Tuple z x) (Tuple z y) -> Circuit x y *)
-
-(*   | Map: forall x y n, Circuit x y -> Circuit (Vector x n) (Vector y n) *)
-(*   | Resize: forall x n nn, Circuit (Vector x n) (Vector x nn) *)
 
 Import VectorNotations.
 Import KappaNotation.
@@ -178,13 +110,24 @@ Definition canright_composed
   let decoded = !aes_sbox_canright !CIPH_INV encoded in
   decoded ]>.
 
-Definition obeys_spec {i o}
-           (c : @morphism Kind KappaCat i o)
-           (spec : denote_kind i -> denote_kind o) :=
-  circuit_equiv _ _ (closure_conversion' Datatypes.nil (c natvar))
-                (fun (x : denote_kind (i ** as_kind Datatypes.nil)%Arrow) =>
-                   spec (Datatypes.fst x)).
+Require Import Coq.derive.Derive.
 
+Derive CIPH_FWD_spec
+       SuchThat (obeys_spec CIPH_FWD CIPH_FWD_spec)
+       As CIPH_FWD_correct.
+Proof.
+  cbv [CIPH_FWD]. circuit_spec.
+  subst CIPH_FWD_spec.
+  instantiate_app_by_reflexivity.
+Qed.
+
+(* This lemma could also be proved the same way as CIPH_FWD *)
+Lemma CIPH_INV_correct : obeys_spec CIPH_INV (fun _ => true).
+Proof.
+  cbv [obeys_spec CIPH_INV]. circuit_spec. reflexivity.
+Qed.
+
+(* TODO: fill in these axioms *)
 Axiom aes_sbox_canright_spec :
   denote_kind (<<Bit, Vector Bit 8, Unit >>) -> denote_kind (Vector Bit 8).
 Axiom aes_sbox_canright_correct :
@@ -192,104 +135,14 @@ Axiom aes_sbox_canright_correct :
 Axiom CircuitLaws : CategoryLaws CircuitCat.
 Existing Instance CircuitLaws.
 
-(* this lemma helps get a subcircuit goal into the [obeys_spec] form so eauto
-recognizes it *)
-Lemma obeys_spec_to_circuit_equiv i o c spec :
-  @obeys_spec i o c spec ->
-  circuit_equiv _ _ (closure_conversion' Datatypes.nil (c natvar))
-                (fun x => spec (Datatypes.fst x)).
-Proof. intro H; exact H. Qed.
-
-Require Import Coq.derive.Derive.
-
-Ltac instantiate_lhs_app_by_reflexivity :=
-  lazymatch goal with
-  | |- ?g ?x = ?rhs =>
-    is_evar g;
-    lazymatch rhs with
-    | context [x] =>
-      match (eval pattern x in rhs) with
-      | ?f _ =>
-        let H := fresh in
-        assert (forall y, f y = g y) as H;
-        [ intros; reflexivity | solve [apply H] ]
-      end
-    | _ =>
-      (* x does not appear on RHS, so ignore the argument *)
-      assert (g = (fun _ => rhs)); reflexivity
-    end
-  | |- ?G => fail "Expected goal of form [?g ?x = ?rhs] (where g must be an evar), got" G
-  end.
-
-Ltac instantiate_rhs_app_by_reflexivity :=
-  symmetry; instantiate_lhs_app_by_reflexivity.
-
-Ltac instantiate_app_by_reflexivity :=
-  first [instantiate_lhs_app_by_reflexivity
-        | instantiate_rhs_app_by_reflexivity ].
-
-Ltac t :=
-  lazymatch goal with
-  | |- ?lhs = ?rhs =>
-    cbn [Datatypes.fst Datatypes.snd];
-    instantiate_app_by_reflexivity
-  | |- circuit_equiv _ _ ?c _ =>
-    lazymatch c with
-    | closure_conversion' _ _ =>
-      (* subcircuit *)
-      apply obeys_spec_to_circuit_equiv; solve [eauto with correctness]
-    | _ => econstructor; intros
-    end
-  | |- ?x => fail "Stuck at" x
-  end.
-
-Hint Unfold cancell cancelr uncancell uncancelr assoc unassoc first second
-     copy drop swap compose
-     CircuitCat CircuitArrow CircuitArrowSwap CircuitArrowDrop CircuitArrowCopy
-     arrow_category as_kind Datatypes.length Nat.eqb extract_nth
-     rewrite_or_default
-  : arrowunfold.
-
-Derive CIPH_FWD_spec
-       SuchThat (obeys_spec CIPH_FWD CIPH_FWD_spec)
-       As CIPH_FWD_correct.
-Proof.
-  cbv [obeys_spec CIPH_FWD]. cbn [closure_conversion'].
-  autounfold with arrowunfold.
-  repeat t.
-
-  cbn [denote_kind combinational_evaluation'] in *.
-  subst CIPH_FWD_spec.
-  instantiate_lhs_app_by_reflexivity.
-Qed.
-
-(* This lemma could also be proved the same way as CIPH_FWD *)
-Lemma CIPH_INV_correct : obeys_spec CIPH_INV (fun _ => true).
-Proof.
-  cbv [obeys_spec CIPH_INV]. cbn [closure_conversion'].
-  autounfold with arrowunfold.
-  repeat t.
-  reflexivity.
-Qed.
-
-(* TODO: replace with upstream resize_default_id *)
-Axiom resize_default_id :
-  forall A n d (v : t A n), resize_default d n v = v.
-
 Hint Resolve aes_sbox_canright_correct CIPH_FWD_correct CIPH_INV_correct
-  : correctness.
+  : circuit_spec_correctness.
 
 Derive canright_composed_spec
        SuchThat (obeys_spec canright_composed canright_composed_spec)
        As canright_composed_correct.
 Proof.
-  intros.
-  cbv [obeys_spec canright_composed].
-  cbn [closure_conversion'].
-  autounfold with arrowunfold.
-
-  repeat t.
-  cbn [denote_kind combinational_evaluation' Datatypes.fst Datatypes.snd].
+  cbv [canright_composed]. circuit_spec.
   rewrite !resize_default_id, !map_id.
   (* we need to do this destruct for the instantiation to work; the calls to
      Datatypes.fst have different types *)
@@ -298,7 +151,8 @@ Proof.
   subst canright_composed_spec.
   instantiate_app_by_reflexivity.
 Qed.
-Print canright_composed_spec.
+(* Uncomment below to see derived spec for canright_composed *)
+(* Print canright_composed_spec. *)
 
 Lemma canright_composed_combinational: is_combinational (closure_conversion aes_sbox_canright).
 Proof. time simply_combinational. Qed.
